separation logic cancellation works

bedrock2/src/Map.v
@@ -25,6 +25,7 @@ Module map.
     (* FIXME: move proofs to a different file *)
     Context {key value} {map : map key value}.
     Context (map_ext : forall m1 m2, (forall k, get m1 k = get m2 k) -> m1 = m2).
+    Context (get_empty : forall k, get empty k = None).
     Context (union_None : forall m1 m2 k, get m2 k = None -> get (union m1 m2) k = get m1 k).
     Context (union_Some : forall m1 m2 k v, get m2 k = Some v -> get (union m1 m2) k = Some v).
     
@@ -39,7 +40,7 @@ Module map.
       { exists v. split. reflexivity. erewrite union_Some; eauto. }
       { split. reflexivity. rewrite union_None; eauto. }
     Qed.
-
+    
     Lemma union_comm x y : disjoint x y -> union x y = union y x.
     Proof.
       cbv [disjoint]; intros; eapply map_ext; intros.
@@ -62,6 +63,11 @@ Module map.
       destruct (get z k) as [?vz|] eqn:?Hz;
       firstorder congruence.
     Qed.
+
+    Lemma union_empty_r x : union x empty = x.
+    Proof. eapply map_ext; intros; rewrite union_None; eauto. Qed.
+    Lemma union_empty_l x : union empty x = x.
+    Proof. rewrite (union_comm empty x) by congruence; eapply union_empty_r. Qed.
     
     Definition split m m1 m2 : Prop :=
       m = (union m1 m2) /\ disjoint m1 m2.
@@ -73,6 +79,8 @@ Module map.
       | cons m0 ms' => carve m0 m (fun m => splits m ms')
       end.
                               
+    Lemma disjoint_empty_l x : disjoint empty x. repeat intro; congruence. Qed.
+    Lemma disjoint_empty_r x : disjoint x empty. repeat intro; congruence. Qed.
     Lemma disjoint_comm m1 m2 : disjoint m1 m2 <-> disjoint m2 m1.
     Proof. cbv [disjoint]. firstorder idtac. Qed.
     Lemma disjoint_union_r x y z : disjoint x (union y z) <-> (disjoint x y /\ disjoint x z).
@@ -95,24 +103,29 @@ Module map.
     Ltac t :=
       repeat match goal with
       | _ => progress subst
-      | _ => progress cbv [split] in *
-      | H:disjoint (union _ _) _ |- _ => 
-        eapply disjoint_union_l in H; destruct H
+      | H:_ /\ _ |- _ => destruct H
+      | H:exists _, _ |- _ => destruct H
+      | H:disjoint (union _ _) _ |- _ => eapply disjoint_union_l in H; destruct H
+      | H:disjoint _ (union _ _) |- _ => eapply disjoint_union_r in H; destruct H
       | _ => progress intuition idtac
+      end.
+
+    Ltac carve_comm_t := repeat match goal with
+      | _ => progress t
       | |- union (union ?a ?b) ?c = union (union ?a ?c) ?b  =>
         rewrite <-2union_assoc by eauto using (fun m1 m2 => proj2 (disjoint_comm m1 m2));
         rewrite (union_comm b c) by eauto using ((fun m1 m2 m3 => proj2 (disjoint_union_r m1 m2 m3)));
         reflexivity
       | _ => solve [eauto using ((fun m1 m2 m3 => proj2 (disjoint_union_r m1 m2 m3))), (fun m1 m2 => proj2 (disjoint_comm m1 m2))]
       | _ => solve [eapply union_comm; eauto using ((fun m1 m2 m3 => proj2 (disjoint_union_r m1 m2 m3))), (fun m1 m2 => proj2 (disjoint_comm m1 m2))]
-      end.
-
+    end.
+    
     Lemma carve_comm x y m l :
       carve y m (fun m_y : rep => carve x m_y (fun m_xy : rep => splits m_xy l)) <->
       carve x m (fun m_x : rep => carve y m_x (fun m_xy : rep => splits m_xy l)).
     Proof.
-      cbv [carve]; split; intros (? & (? & (? & ? & ?)) );
-        match goal with M : rep, z : rep |- _ => solve [exists (union M z); t] end.
+      cbv [carve split]; split; intros (? & (? & (? & ? & ?)) );
+        match goal with M : rep, z : rep |- _ => solve [exists (union M z); carve_comm_t] end.
     Qed.
 
     Require Import Permutation.
@@ -121,6 +134,107 @@ Module map.
     Proof.
       cbv [Proper respectful]; intros x y H; revert m; induction H; intros;
         try solve [ eapply carve_comm | firstorder idtac ].
+    Qed.
+
+    Definition impl1 {T} (P Q:_->Prop) : Prop := forall x:T, P x -> Q x.
+    Global Instance Transitive_impl1 T : Transitive (@impl1 T). firstorder idtac. Qed.
+    Global Instance Reflexive_impl1 T : Reflexive (@impl1 T). firstorder idtac. Qed.
+    Global Instance Proper_impl1_impl1 T : Proper (Basics.flip impl1 ==> impl1 ==> Basics.impl) (@impl1 T). firstorder idtac. Qed.
+    Definition iff1 {T} (P Q:_->Prop) : Prop := forall x:T, P x <-> Q x.
+    Global Instance subrelation_iff1_impl1 T : subrelation (@iff1 T) (@impl1 T). firstorder idtac. Qed.
+    Global Instance Equivalence_iff1 T : Equivalence (@iff1 T). firstorder idtac. Qed.
+    Global Instance Proper_iff1_iff1 T : Proper (iff1 ==> iff1 ==> iff) (@iff1 T). firstorder idtac. Qed.
+    Global Instance Proper_iff1_impl1 T : Proper (Basics.flip impl1 ==> impl1 ==> Basics.impl) (@impl1 T). firstorder idtac. Qed.
+    Global Instance Proper_impl1_iff1 T : Proper (iff1 ==> iff1 ==> iff) (@impl1 T). firstorder idtac. Qed.
+    Definition emp (P : Prop) := fun m => m = empty /\ P.
+    Global Instance Proper_emp_iff : Proper (iff ==> iff1) emp. firstorder idtac. Qed.
+    Global Instance Proper_emp_impl : Proper (Basics.impl ==> impl1) emp. firstorder idtac. Qed.
+    Definition sep (p q : rep -> Prop) m :=
+      exists mp mq, split m mp mq /\ p mp /\ q mq.
+    Local Infix "*" := sep.
+    Global Instance Proper_sep_iff1 : Proper (iff1 ==> iff1 ==> iff1) sep. firstorder idtac. Qed.
+    Global Instance Proper_sep_impl1 : Proper (impl1 ==> impl1 ==> impl1) sep. firstorder idtac. Qed.
+    Definition ptsto k v := fun m => m = put empty k v.
+    Definition exi {T} (P : T -> rep -> Prop) := fun m => exists x:T, P x m.
+    Global Instance Proper_exi_iff1 T : Proper (pointwise_relation _ iff1 ==> iff1) (@exi T). firstorder idtac. Qed.
+    Global Instance Proper_exi_impl1 T : Proper (pointwise_relation _ impl1 ==> impl1) (@exi T). firstorder idtac. Qed.
+    Definition read k (P : value -> rep -> Prop) := (exi (fun v => ptsto k v * P v)).
+    
+
+    Lemma sep_comm p q : iff1 (p*q) (q*p).
+    Proof. cbv [iff1 sep split]; firstorder (subst; eauto using union_comm). Qed.
+    Lemma sep_assoc p q r : iff1 ((p*q)*r) (p*(q*r)).
+    Proof. cbv [iff1 sep split]; split; t;
+           eauto 15 using eq_sym, union_assoc, ((fun m1 m2 m3 => proj2 (disjoint_union_l m1 m2 m3))), ((fun m1 m2 m3 => proj2 (disjoint_union_r m1 m2 m3))).
+    Qed.
+    Lemma sep_cancel (p1 p2 q1 q2:_->Prop) (_:impl1 p1 p2) (_:impl1 q1 q2) : impl1 (p1*q1) (p2*q2).
+    Proof. cbv [impl1 sep]; firstorder idtac. Qed.
+    Lemma sep_emp_emp p q : iff1 (sep (emp p) (emp q)) (emp (p /\ q)).
+    Proof. cbv [iff1 sep emp split]; t; intuition eauto 20 using union_empty_l, disjoint_empty_l. Qed.
+    Lemma sep_exi_r {T} p q : iff1 (p * @exi T q) (exi (fun h => p * q h)).
+    Proof. cbv [exi sep]; firstorder idtac. Qed.
+    Lemma sep_exi_l {T} p q : iff1 (@exi T q * p) (exi (fun h => q h * p)).
+    Proof. rewrite sep_comm. rewrite sep_exi_r. setoid_rewrite (sep_comm p). reflexivity. Qed.
+    Lemma impl1_exi_l {T} p q : impl1 (exi p) q <-> (forall x:T, impl1 (p x) q).
+    Proof. cbv [exi sep impl1]; firstorder idtac. Qed.
+    Lemma impl1_exi_r {T} p q (x:T) : impl1 p (q x) -> impl1 p (exi q).
+    Proof. cbv [exi sep impl1]; firstorder idtac. Qed.
+
+    Lemma sep_213 B A C : iff1 (A * (B * C)) (B * (A * C)).
+    Proof. rewrite <-(fun a b => sep_assoc a B b), (fun a => sep_comm a B), sep_assoc. reflexivity. Qed.
+    Lemma sep_emp_r a b : iff1 (a * emp b) (emp b * a). eapply sep_comm. Qed.
+    Lemma sep_emp_2 a b c : iff1 (a * (emp b * c)) (emp b * (a * c)).
+    Proof. rewrite <-sep_assoc. rewrite (sep_comm a). rewrite sep_assoc. reflexivity. Qed.
+    Lemma sep_emp_12 a b c : iff1 (emp a * (emp b * c)) (emp (a /\ b) * c).
+    Proof. rewrite <-sep_assoc. rewrite sep_emp_emp. reflexivity. Qed.
+
+    Lemma impl1_l_sep_emp (a:Prop) b c : impl1 (emp a * b) c <-> (a -> impl1 b c).
+    Proof.
+      cbv [impl1 emp sep split]. firstorder idtac; subst; rewrite ?union_empty_l; eauto.
+      eapply H. exists empty, x.  rewrite union_empty_l. repeat split; eauto using disjoint_empty_l.
+    Qed.
+
+    Lemma impl1_r_sep_emp a b c : (b /\ impl1 a c) -> impl1 a (emp b * c).
+    Proof.
+      cbv [impl1 emp sep split]. firstorder idtac; subst.
+      exists empty, x. rewrite union_empty_l. repeat split; eauto using disjoint_empty_l.
+    Qed.
+
+    Ltac set_evars := repeat match goal with |- context[?e] => is_evar e; set e end.
+    Ltac subst_evars := repeat match goal with x := ?e |- _ => is_evar e; subst x end.
+    Ltac normalize :=
+      set_evars;
+      repeat (rewrite_strat (bottomup (terms @sep_emp_emp @sep_emp_r @sep_emp_12 @sep_emp_2 @sep_exi_l @sep_exi_r @sep_assoc)));
+      subst_evars.
+    Ltac cancel_atom_goal1 P :=
+      (* COQBUG: if I use fresh here, rewrite_strat fails *)
+      pose proof (sep_213 P) as _cancel_atom_goal1_ASDA;
+      (rewrite_strat (try (bottomup (terms _cancel_atom_goal1_ASDA))));
+      clear _cancel_atom_goal1_ASDA.
+    Ltac cancel_atom P :=
+      eapply Proper_impl1_impl1; [ cbv [Basics.flip]; cancel_atom_goal1 P; eapply (Proper_sep_impl1 P _ (reflexivity _)) | reflexivity | reflexivity ].
+    Ltac cancel :=
+      lazymatch goal with |- impl1 _ (_ * _) => idtac end;
+      set_evars;
+      repeat match goal with |- impl1 _ (?P * _) => cancel_atom P end;
+      subst_evars.
+
+    Goal forall A B C D E, exists R, impl1 (A*emp True*B*exi(fun x:unit => C*(exi (fun v : value => (emp (x = x)* emp(v =v))*E v x)))*D) (A * exi (fun n => C * emp (1=n)) * R).
+    Proof.
+      intros.
+      normalize.
+      eexists ?[R].
+      eapply impl1_exi_r.
+      eapply impl1_r_sep_emp.
+      split. reflexivity.
+      apply impl1_exi_l. intros.
+      apply impl1_exi_l. intros.
+      apply impl1_l_sep_emp. intros.
+      cancel.
+      instantiate (1 := exi (fun x0 => exi (fun x => (B * (E x0 x * D))))).
+      eapply impl1_exi_r.
+      eapply impl1_exi_r.
+      reflexivity.
     Qed.
   End Properties.
   
